Test/Tactics/Skolemizatoin.lean
@@ -1,0 +1,8 @@
+import Auto.Tactic
+
+set_option trace.auto.lamReif.printResult true in
+example (p q : α → Prop) (h₁ : ∃ f, p f) (h₂ : ∀ f, p f → q f) : ∃ f, q f :=
+  by auto [*]
+
+set_option trace.auto.lamReif.printResult true in
+example (α : Prop) (h₁ : α) (h₂ : α) : α := by auto
